LeanGrow/Src/SampleGenScore/Docs/Split.lean
@@ -8,3 +8,95 @@ open Lean Meta Elab Tactic
 #check evalSplit
 
 #check_failure Mathlib.Tactic.splitIfsCore
+
+
+theorem test_1 (n : Nat) :
+  (match n with
+  | 0 => 1
+  | 1 => 37
+  | n+2 => n
+    ) = 42 := by
+      split
+      all_goals sorry
+
+set_option pp.privateNames true in
+#print test_1
+#print test_1.match_1.splitter
+
+set_option pp.privateNames true in
+#check test_1
+
+#print MatcherInfo
+#print Match.MatchEqns
+
+#eval ((do let env ← getEnv ; return Match.isMatchEqnTheorem env `test_1.match_1.splitter) : CoreM Bool)
+
+def isMatchSpliiter (env : Environment) : Array (Name × Name) := Id.run do
+  return (Match.matchEqnsExt.getState (asyncMode := .async .asyncEnv)  env).map.toArray.map (fun (x,y) => (x,y.splitterName))
+
+
+#eval ((do let env ← getEnv ; return isMatchSpliiter env ) : CoreM _)
+
+#check 1
+
+#eval ((do let eqs ← Match.getEquationsFor `test_1.match_1 ; return eqs.splitterName) : MetaM _)
+
+#eval ((do let eqs ← Match.getEquationsFor `test_1.match_1 ; return eqs.splitterAltNumParams) : MetaM _)
+
+
+#check 1
+--splitterAltNumParams
+
+theorem test_2 (n : Nat) (h : n + 5 = 10) :
+  (match n+1 with
+  | 0 => 1
+  | 1 => 67
+  | 3 => 42
+  | n+2 => n
+    ) = 42 + (n+1) := by
+      split
+      all_goals sorry
+
+#print test_2
+
+
+theorem test_3 (n : Nat) :
+  (match n with
+  | 0 => 1
+  | n+1 => if n = 67 then 42 else 666
+    ) = if n = 67 then 42 else 666 := by
+      split
+      all_goals sorry
+
+#print test_3
+
+theorem test_4 (n : Nat) :
+  37 = if n = 67 then 42 else 666 := by
+    split
+    all_goals sorry
+
+#print test_4
+
+open Classical in
+theorem test_5 (n : Nat) :
+  37 = if (∃ m, n = 67 +m) then 42 else 666 := by
+    split
+    all_goals sorry
+
+#print test_5
+
+
+theorem test_6 (n : Nat) :
+  37 = if n = 67 then 42 else 666 := by
+    split_ifs
+    all_goals sorry
+
+#print test_6
+
+open Classical in
+theorem test_7 (n : Nat) :
+  37 = if (∃ m, n = 67 +m) then 42 else 666 := by
+    split_ifs
+    all_goals sorry
+
+#print test_7
